src/ntac/goal_tree.lean
@@ -1,4 +1,5 @@
 import ntac.semantic_tree
+import ntac.ja
 
 meta structure type_info := (type: expr) (kind: expr)
 meta structure named_expr := (name: name) (type: expr) (kind: expr)
@@ -33,15 +34,7 @@ with goal_tree : Type
 | init : goal_info → goal_tree
 | andthen : goal_tree →list (expr × goal_info) → goal_tree
 
--- meta def juststr (s: string): goal_tree := goal_tree.tact [([], λ _,s)]
--- meta def goal_tree1 (g: goal_tree) (f: string → string): goal_tree := goal_tree.tact [g] (λ p, 
--- match p with 
--- | h::[]  := f h
--- |_ := "error!"
--- end)
--- meta def addtact (g: goal_tree) (s: string) := goal_tree1 g (λ st, st ++ s)
-
-meta def replc_unres :expr → goal_tree → goal_tree → goal_tree := 
+meta def replc_unres :expr → goal_tree → goal_info → goal_info := 
 λ e g_new g_org,
 let rep_info : goal_info → goal_info := (λ gi, match gi with | goal_info.mk ty g := goal_info.mk ty (replc_unres e g_new g) end)
 in
@@ -95,53 +88,70 @@ meta def goal_tree_to_semantic_tree : goal_tree → semantic_tree :=
 | goal_tree.simp2 ln g:= semantic_tree.unresolved
 | goal_tree.simp g:= semantic_tree.unresolved
 | goal_tree.skip  (goal_info.mk a g):= goal_tree_to_semantic_tree g
-| goal_tree.apply ee gl := semantic_tree.unresolved
+| goal_tree.apply ee gl := match ee with
+    | `(Exists.intro %%n) := 
+    |_ :=semantic_tree.unresolved
+  end
 | goal_tree.case gl := semantic_tree.unresolved
 | goal_tree.andthen gl l:= semantic_tree.unresolved
 | goal_tree.init (goal_info.mk a g) := semantic_tree.init $ goal_tree_to_semantic_tree g
 end
+#check ([1,1] ++ [1,2] )++ [3,2]
+meta def join_expr (ts:tactic string) (e:expr ): tactic string :=
+do ppe ← tactic.pp e,
+s ← ts,
+return $ s ++ ppe.to_string
+meta def join_expr2 (ts:tactic string) (e:expr ): tactic string :=
+do s ← ts,
+return $ s ++ e.to_string
 
-
-meta def goal_tree_to_string : goal_tree → string :=
-let goal_tree_to_string2: goal_info → string := λ gi, match gi with goal_info.mk ty g := goal_tree_to_string g end in
-let goal_tree_to_string3: goal_info → string := λ gi, match gi with goal_info.mk ty g := "("++(to_string ty.type) ++"::" ++(goal_tree_to_string g)++")" end in
+meta def join_str :tactic string→ string → tactic string := flip $ λ e, functor.map (++e) 
+meta def join_tstr (ts1 : tactic string) (ts2 : tactic string) : tactic string := do 
+s1 ← ts1, s2 ← ts2, return (s1++s2)
+local infix `+S+`:65 := join_str
+local infix `+E+`:65 := join_expr
+local infix `+T+`:65 := join_tstr
+local prefix `!`:75 := return
+meta def goal_tree_to_string : goal_tree → tactic string :=
+let goal_tree_to_string2: goal_info → tactic string := λ gi, match gi with goal_info.mk ty g := goal_tree_to_string g end in
+let goal_tree_to_string3: goal_info → tactic string := λ gi, match gi with goal_info.mk ty g := do ty ← tactic.pp ty.type,g ← (goal_tree_to_string g),return $ "("++ty.to_string++"::" ++g++")" end in
 λ g, match g with
-| goal_tree.unres e :=  " *unres* :"++e.to_string
-| goal_tree.unres_andthen e :=  " *unres andthen* :"++e.to_string
-| goal_tree.admit := "sorry"
-| goal_tree.intro (n, e) g := "INTRO " ++ to_string n ++ ":" ++ to_string e ++ "(" ++ (goal_tree_to_string2 g) ++ ")"
-| goal_tree.have_ ⟨name, type, kind, val⟩ g := "have " ++ type.to_string ++ "by <"++val.to_string ++">"++"and"++ "<" ++ (goal_tree_to_string2 g) ++ ">"
-| goal_tree.define edef eval g := "let " ++ edef.to_string++" := " ++ eval.to_string ++ ">" ++"and"++ "<" ++ (goal_tree_to_string2 g) ++ ">"
-| goal_tree.willhave ⟨name, type, kind⟩ newg oldg := "will have " ++ type.to_string ++" from" ++ "<" ++ (goal_tree_to_string2 newg) ++ ">" ++"and"++ "<" ++ (goal_tree_to_string2 oldg) ++ ">"
-| goal_tree.suffice ⟨name, type, kind⟩ newg oldg := "suffice " ++ type.to_string ++" from"  ++ "<" ++ (goal_tree_to_string2 newg) ++ ">" ++"and"++ "<" ++ (goal_tree_to_string2 oldg) ++ ">"
-| goal_tree.willdefine e newg oldg := "will let" ++ e.to_string++"by" ++ "<" ++ (goal_tree_to_string2 newg) ++ ">" ++"and"++ "<" ++ (goal_tree_to_string2 oldg) ++ ">"
-| goal_tree.done := "done"
-| goal_tree.exact e:= "exact " ++e.to_string 
-| goal_tree.triv g:= "triv (" ++goal_tree_to_string2 g ++ ")"
-| goal_tree.existsi e g:= "exists (" ++ e.to_string ++ "and indeed"++goal_tree_to_string2 g ++ ")"
-| goal_tree.assumption e:= "assumption " ++e.to_string 
-| goal_tree.contra g:= "contradiction (" ++ goal_tree_to_string2 g ++")"
-| goal_tree.rewrite g:= "rw (" ++ goal_tree_to_string2 g ++")"
-| goal_tree.simp2 ln g:= "simp by "++string.join (list.map to_string ln) ++"(" ++ goal_tree_to_string2 g ++")" 
-| goal_tree.simp (some g):= "simp (" ++ goal_tree_to_string2 g ++")" 
-| goal_tree.simp none:= "by simp" 
-| goal_tree.skip g:= "skip (" ++ goal_tree_to_string2 g ++ ")"
+| goal_tree.unres e := !" *unres* :"+E+e
+| goal_tree.unres_andthen e := !" *unres andthen* :"+E+e
+| goal_tree.admit := !"sorry"
+| goal_tree.intro (n, e) g := !"INTRO " +S+ to_string n +S+ ":" +E+ e +S+ "(" +T+ (goal_tree_to_string2 g) +S+ ")"
+| goal_tree.have_ ⟨name, type, kind, val⟩ g := !"have " +E+ type +S+ "by <"+E+ val +S+ ">and<" +T+ (goal_tree_to_string2 g) +S+ ">"
+| goal_tree.define edef eval g := !"let "+E+ edef +S+" := " +E+ eval +S+ ">and<" +T+ (goal_tree_to_string2 g) +S+ ">"
+| goal_tree.willhave ⟨name, type, kind⟩ newg oldg := !"will have " +E+ type +S+" from<" +T+ (goal_tree_to_string2 newg) +S+ ">and<" +T+ (goal_tree_to_string2 oldg) +S+ ">"
+| goal_tree.suffice ⟨name, type, kind⟩ newg oldg := !"suffice " +E+ type +S+" from<" +T+ (goal_tree_to_string2 newg) +S+ ">and<" +T+ (goal_tree_to_string2 oldg) +S+ ">"
+| goal_tree.willdefine e newg oldg := !"will let" +E+ e +S+ "by<" +T+ (goal_tree_to_string2 newg) +S+ ">and<" +T+ (goal_tree_to_string2 oldg) +S+ ">"
+| goal_tree.done := !"done"
+| goal_tree.exact e:= !"exact " +E+ e
+| goal_tree.triv g:= !"triv (" +T+ goal_tree_to_string2 g +S+ ")"
+| goal_tree.existsi e g:= !"exists (" +E+ e +S+ "and indeed" +T+ goal_tree_to_string2 g +S+ ")"
+| goal_tree.assumption e:= !"assumption " +E+ e
+| goal_tree.contra g:= !"contradiction (" +T+ goal_tree_to_string2 g +S+")"
+| goal_tree.rewrite g:= !"rw (" +T+ goal_tree_to_string2 g +S+")"
+| goal_tree.simp2 ln g:= !"simp by "+S+string.join (list.map to_string ln) +S+"(" +T+ goal_tree_to_string2 g +S+")" 
+| goal_tree.simp (some g):= !"simp (" +T+ goal_tree_to_string2 g +S+")" 
+| goal_tree.simp none:= !"by simp" 
+| goal_tree.skip g:= !"skip (" +T+ goal_tree_to_string2 g +S+ ")"
 | goal_tree.apply ee gl := 
 let sl := list.map goal_tree_to_string3 gl in
-let str := list.foldl (λ acc s, acc ++", "++ s) ("apply <" ++ee.to_string ++"> and from[") sl in
-str ++ "]"
+let str := list.foldl (λ acc s, acc +S+", "+T+ s) (!"apply <" +E+ee +S+"> and from[") sl in
+str +S+ "]"
 | goal_tree.case gl := 
 let sl := list.map goal_tree_to_string3 gl in
-let str := list.foldl (λ acc s, acc ++", "++ s) "case[" sl in
-str ++ "]"
-  
-| goal_tree.init g := "init[" ++ goal_tree_to_string2 g ++ "]"
+let str := list.foldl (λ acc s, acc +S+", "+T+ s) (!"case[") sl in
+str +S+ "]"
+
+| goal_tree.init g := !"init[" +T+ goal_tree_to_string2 g +S+ "]"
 
 | goal_tree.andthen tac1 tac2 :=
 let str1 := goal_tree_to_string tac1 in
-let sl := @list.map (expr × goal_info) string (λ p, let (a, b) := p in "("++(to_string a) ++" → " ++(goal_tree_to_string2 b)++")") tac2 in
-let str := list.foldl (λ acc s, acc ++", "++ s) ("do {"++str1++"} and then{") sl in
-str ++ "}"
+let sl := @list.map (expr × goal_info) (tactic string) (λ p, let (a, b) := p in !"("+E+a +S+" → " +T+(goal_tree_to_string2 b)+S+")") tac2 in
+let str := list.foldl (λ acc s, acc +S+", "+T+ s) (!"do {"+T+str1+S+"} and then{") sl in
+str +S+ "}"
 end
 
 meta def for_andthen : goal_tree → goal_tree :=
@@ -149,7 +159,10 @@ meta def for_andthen : goal_tree → goal_tree :=
 | goal_tree.unres e := goal_tree.unres_andthen e
 | _ := g
 end
-
-meta instance : has_to_format goal_tree :=
-⟨λ g,to_fmt $ goal_tree_to_string g⟩
+meta def goal_tree_to_format : goal_tree → tactic format :=
+λ g, do str ← goal_tree_to_string g,return $ to_fmt str
+meta def goal_tree_to_format2 : goal_tree → tactic format :=
+λ g, return $ to_fmt $ list.map S_ja $ tolistS $ goal_tree_to_semantic_tree $ g
+meta instance : has_to_tactic_format goal_tree :=
+⟨goal_tree_to_format⟩
 
