src/ntac/semantic_tree.lean
@@ -1,4 +1,4 @@
-import ntac.statement
+import ntac.sentence
 
 
 meta inductive semantic_tree : Type
@@ -17,10 +17,17 @@ meta inductive semantic_tree : Type
 | contra : semantic_tree → semantic_tree
 | init : semantic_tree → semantic_tree
 
-meta def semantic_tree_to_list_statement : semantic_tree → list statement :=
+meta def tolistS : semantic_tree → list S :=
 λ s,match s with
-| semantic_tree.trivial := [statement.trivial]
-| semantic_tree.suffice_from p s := "dfdfd"
-| semantic_tree.have_from p v s := "df"
-| _ := "fg"
-  end
+| semantic_tree.trivial := [S._trivial]
+| semantic_tree.init s := tolistS s
+| semantic_tree.suffice_from e t1 t2 :=tolistS t1 ++ Adv._hence /a/ <eNP>e /p/ <VVP>V._suf_show :: tolistS t2
+| semantic_tree.have_from t1 t2 := tolistS t1 ++ tolistS t2
+| semantic_tree.assume_prop e t:= /i/ <V2VP>V2._assume <eNP>e :: tolistS t
+| semantic_tree.exact e := [Adv._from_assum /a/ <S>e]
+| semantic_tree.assume_val edef eval t:= /i/ <V3VP> V3._let <NP><eN>edef <NP><eN>eval :: tolistS t
+| semantic_tree.assume_exist e t := [S._trivial]
+| semantic_tree.have_exact e t := Adv._from <NP><eN>e /a/ S._trivial :: tolistS t
+| semantic_tree.let_from t1 t2 := tolistS t1 ++ tolistS t2
+| _ :=[S._trivial]
+end
