src/ntac/sentence.lean
@@ -1,0 +1,49 @@
+inductive prop : Type
+| noun : prop
+
+
+meta mutual inductive S, NP, N, VP, V, V2, V3, Subj, Adv
+with S : Type
+| AdvS : Adv → S → S
+| AdvS' : S → Adv → S
+| Expr : expr → S
+| PredVP : NP → VP → S
+| _trivial : S
+| Imp : VP → S
+with NP : Type
+| EmbedS : S → NP
+| UseN : N → NP
+with N: Type
+| Expr : expr → N
+with VP : Type
+| UseV : V → VP
+| UseV2 : V2 → NP → VP
+| UseV3 : V3 → NP → NP → VP
+with V : Type
+| _suf_show : V
+with V2: Type
+| _assume : V2
+with V3: Type
+| _let : V3
+with Subj : Type
+| _if : Subj
+with Adv : Type
+| Subjs : Subj → S → Adv
+| _from : NP → Adv
+| _hence : Adv
+| _from_assum : Adv
+infix `/a/`:140 := S.AdvS
+infix `/aa/`:140 := S.AdvS'
+infix `/p/`:160 := S.PredVP
+prefix `/i/`:110 := S.Imp
+infix `/s/`:150 := Adv.Subjs
+prefix `<eNP>`:200 := λ e, NP.EmbedS (S.Expr e)
+prefix `<eN>`:200 := N.Expr
+prefix `<NP>`:190 := NP.UseN
+prefix `<S>`:200 := S.Expr
+prefix `<VVP>`:300 := VP.UseV
+prefix `<V2VP>`:300 := VP.UseV2
+prefix `<V3VP>`:300 := VP.UseV3
+
+--the precedence of ++ is 65
+--the precedence of :: is 67
