src/ntac/statement.lean
@@ -1,7 +1,0 @@
-inductive prop : Type
-| noun : prop
-
-meta inductive statement : Type
-| trivial : statement
-
-
